theories/TransformerLens/HookedTransformer/Instances.v
@@ -23,7 +23,7 @@ Local Open Scope raw_tensor_scope.
 
 Module HookedTransformer.
   Export HookedTransformer.
-Print Reduction.sum.
+
   Ltac t_step :=
     first [ match goal with
             | [ |- ?x = ?x ] => reflexivity
@@ -163,7 +163,6 @@ Print Reduction.sum.
   Module PosEmbed.
     Export PosEmbed.
 
-    Print forward.
     #[export] Instance forward_Proper_dep {r batch_pos tokens_length d_model n_ctx}
       : Dependent.Proper
           (Tensor.eqfR
@@ -320,31 +319,6 @@ Print Reduction.sum.
       : Proper (Tensor.eqf ==> Tensor.eqf) (@v A r batch addA zeroA mulA defaultA pos n_heads d_model d_head use_split_qkv_input W_V b_V).
     Proof. apply v_Proper_dep; repeat intro; subst; reflexivity. Qed.
 
-    Print attn_scores.
-    (* attn_scores =
-fun (r : Rank) (batch : Shape r) (pos n_heads d_model d_head : ShapeType) (use_split_qkv_input : with_default "use_split_qkv_input" false) (A : Type) (sqrtA : has_sqrt A) (coerZ : has_coer Z A) (addA : has_add A) (zeroA : has_zero A) (mulA : has_mul A) (divA : has_div A) (defaultA : pointed A) (W_Q W_K : tensor [n_heads; d_model; d_head] A)
-  (b_Q b_K : tensor [n_heads; d_head] A) =>
-let attn_scale := √(coer φ (d_head)) in
-let maybe_n_heads := fun b : bool => if b as b0 return (Shape (if b0 then 1%nat else 0%nat)) then [n_heads]%shape else []%shape in
-fun query_input key_input : tensor (batch ::' pos ++' (maybe_n_heads use_split_qkv_input ::' d_model)) A =>
-let qk := map2' (fun q k : tensor [pos; n_heads; d_head] A => (fun '(tt, i1, i0, i) => ∑_(0≤d_head1<d_head)q.[[i0; i1; d_head1]] * k.[[i; i1; d_head1]]) : tensor [n_heads; pos; pos] A) (q W_Q b_Q query_input) (k W_K b_K key_input) in PArray.checkpoint (qk / broadcast' attn_scale)%core
-     : forall (r : Rank) (batch : Shape r) (pos n_heads d_model d_head : ShapeType) (use_split_qkv_input : with_default "use_split_qkv_input" false) (A : Type),
-       has_sqrt A ->
-       has_coer Z A ->
-       has_add A ->
-       has_zero A ->
-       has_mul A ->
-       has_div A ->
-       pointed A ->
-       tensor [n_heads; d_model; d_head] A ->
-       tensor [n_heads; d_model; d_head] A ->
-       tensor [n_heads; d_head] A ->
-       tensor [n_heads; d_head] A ->
-       tensor (batch ::' pos ++' ((fun b : bool => if b as b0 return (Shape (if b0 then 1%nat else 0%nat)) then [n_heads]%shape else []%shape) use_split_qkv_input ::' d_model)) A ->
-       tensor (batch ::' pos ++' ((fun b : bool => if b as b0 return (Shape (if b0 then 1%nat else 0%nat)) then [n_heads]%shape else []%shape) use_split_qkv_input ::' d_model)) A -> tensor (batch ::' n_heads ::' pos ::' pos) A
-
-Arguments attn_scores {r}%nat_scope {batch}%shape_scope {pos n_heads d_model d_head}%uint63_scope {use_split_qkv_input} {A}%type_scope {sqrtA coerZ addA zeroA mulA divA defaultA} (W_Q W_K b_Q b_K query_input key_input)%tensor_scope _
-*)
     #[export] Instance attn_scores_Proper_dep {r batch pos n_heads d_model d_head use_split_qkv_input}
       : Dependent.Proper
           ((Dependent.idR ==> Dependent.idR)
@@ -380,27 +354,6 @@ Arguments attn_scores {r}%nat_scope {batch}%shape_scope {pos n_heads d_model d_h
       : Proper (Tensor.eqf ==> Tensor.eqf) (@apply_causal_mask r batch pos n_heads n_ctx A coerZ).
     Proof. apply apply_causal_mask_Proper_dep; repeat intro; subst; reflexivity. Qed.
 
-    Print masked_attn_scores.
-    (*
-masked_attn_scores =
-fun (r : Rank) (batch : Shape r) (pos n_heads d_model d_head : ShapeType) (n_ctx : N) (use_split_qkv_input : with_default "use_split_qkv_input" false) (A : Type) (sqrtA : has_sqrt A) (coerZ : has_coer Z A) (addA : has_add A) (zeroA : has_zero A) (mulA : has_mul A) (divA : has_div A) (defaultA : pointed A) (W_Q W_K : tensor [n_heads; d_model; d_head] A) (b_Q b_K : tensor [n_heads; d_head] A) =>
-let IGNORE := coerZ (-1 * 10 ^ 5)%Z in let attn_scale := √(coer φ (d_head)) in let maybe_n_heads := fun b : bool => if b as b0 return (Shape (if b0 then 1%nat else 0%nat)) then [n_heads]%shape else []%shape in fun query_input key_input : tensor (batch ::' pos ++' (maybe_n_heads use_split_qkv_input ::' d_model)) A => let mask := to_bool (tril (ones [of_Z n_ctx; of_Z n_ctx])) in apply_causal_mask (attn_scores W_Q W_K b_Q b_K query_input key_input)
-     : forall (r : Rank) (batch : Shape r) (pos n_heads d_model d_head : ShapeType),
-       N ->
-       forall (use_split_qkv_input : with_default "use_split_qkv_input" false) (A : Type),
-       has_sqrt A ->
-       has_coer Z A ->
-       has_add A ->
-       has_zero A ->
-       has_mul A ->
-       has_div A ->
-       pointed A ->
-       tensor [n_heads; d_model; d_head] A ->
-       tensor [n_heads; d_model; d_head] A ->
-       tensor [n_heads; d_head] A -> tensor [n_heads; d_head] A -> tensor (batch ::' pos ++' ((fun b : bool => if b as b0 return (Shape (if b0 then 1%nat else 0%nat)) then [n_heads]%shape else []%shape) use_split_qkv_input ::' d_model)) A -> tensor (batch ::' pos ++' ((fun b : bool => if b as b0 return (Shape (if b0 then 1%nat else 0%nat)) then [n_heads]%shape else []%shape) use_split_qkv_input ::' d_model)) A -> tensor (batch ::' n_heads ::' pos ::' pos) A
-
-Arguments masked_attn_scores {r}%nat_scope {batch}%shape_scope {pos n_heads d_model d_head}%uint63_scope {n_ctx}%N_scope {use_split_qkv_input} {A}%type_scope {sqrtA coerZ addA zeroA mulA divA defaultA} (W_Q W_K b_Q b_K query_input key_input)%tensor_scope _
-     *)
     #[export] Instance masked_attn_scores_Proper_dep {r batch pos n_heads d_model d_head n_ctx use_split_qkv_input}
       : Dependent.Proper
           ((Dependent.idR ==> Dependent.idR)
@@ -424,44 +377,6 @@ Arguments masked_attn_scores {r}%nat_scope {batch}%shape_scope {pos n_heads d_mo
       : Proper (Tensor.eqf ==> Tensor.eqf ==> Tensor.eqf) (@masked_attn_scores r batch pos n_heads d_model d_head n_ctx use_split_qkv_input A sqrtA coerZ addA zeroA mulA divA defaultA W_Q W_K b_Q b_K).
     Proof. apply masked_attn_scores_Proper_dep; repeat intro; subst; reflexivity. Qed.
 
-    Print pattern.
-    (* pattern =
-fun (r : Rank) (batch : Shape r) (pos n_heads d_model d_head : ShapeType) (n_ctx : N) (use_split_qkv_input : with_default "use_split_qkv_input" false)
-  (A : Type) (sqrtA : has_sqrt A) (coerZ : has_coer Z A) (addA : has_add A) (zeroA : has_zero A) (mulA : has_mul A) (divA : has_div A)
-  (expA : has_exp A) (defaultA : pointed A) (W_Q W_K : tensor [n_heads; d_model; d_head] A) (b_Q b_K : tensor [n_heads; d_head] A) =>
-let IGNORE := coerZ (-1 * 10 ^ 5)%Z in
-let attn_scale := √(coer φ (d_head)) in
-let maybe_n_heads := fun b : bool => if b as b0 return (Shape (if b0 then 1%nat else 0%nat)) then [n_heads]%shape else []%shape in
-fun query_input key_input : tensor (batch ::' pos ++' (maybe_n_heads use_split_qkv_input ::' d_model)) A =>
-let mask := to_bool (tril (ones [of_Z n_ctx; of_Z n_ctx])) in
-PArray.checkpoint (softmax_dim_m1 (masked_attn_scores W_Q W_K b_Q b_K query_input key_input))
-     : forall (r : Rank) (batch : Shape r) (pos n_heads d_model d_head : ShapeType),
-       N ->
-       forall (use_split_qkv_input : with_default "use_split_qkv_input" false) (A : Type),
-       has_sqrt A ->
-       has_coer Z A ->
-       has_add A ->
-       has_zero A ->
-       has_mul A ->
-       has_div A ->
-       has_exp A ->
-       pointed A ->
-       tensor [n_heads; d_model; d_head] A ->
-       tensor [n_heads; d_model; d_head] A ->
-       tensor [n_heads; d_head] A ->
-       tensor [n_heads; d_head] A ->
-       tensor
-         (batch ::' pos ++'
-          ((fun b : bool => if b as b0 return (Shape (if b0 then 1%nat else 0%nat)) then [n_heads]%shape else []%shape) use_split_qkv_input ::' d_model))
-         A ->
-       tensor
-         (batch ::' pos ++'
-          ((fun b : bool => if b as b0 return (Shape (if b0 then 1%nat else 0%nat)) then [n_heads]%shape else []%shape) use_split_qkv_input ::' d_model))
-         A -> tensor (batch ::' n_heads ::' pos ::' pos) A
-
-Arguments pattern {r}%nat_scope {batch}%shape_scope {pos n_heads d_model d_head}%uint63_scope {n_ctx}%N_scope {use_split_qkv_input}
-  {A}%type_scope {sqrtA coerZ addA zeroA mulA divA expA defaultA} (W_Q W_K b_Q b_K query_input key_input)%tensor_scope _
-     *)
     #[export] Instance pattern_Proper_dep {r batch pos n_heads d_model d_head n_ctx use_split_qkv_input}
       : Dependent.Proper
           ((Dependent.idR ==> Dependent.idR)
@@ -485,56 +400,6 @@ Arguments pattern {r}%nat_scope {batch}%shape_scope {pos n_heads d_model d_head}
     #[export] Instance pattern_Proper {r batch pos n_heads d_model d_head n_ctx use_split_qkv_input A sqrtA coerZ addA zeroA mulA divA expA defaultA W_Q W_K b_Q b_K}
       : Proper (Tensor.eqf ==> Tensor.eqf ==> Tensor.eqf) (@pattern r batch pos n_heads d_model d_head n_ctx use_split_qkv_input A sqrtA coerZ addA zeroA mulA divA expA defaultA W_Q W_K b_Q b_K).
     Proof. apply pattern_Proper_dep; repeat intro; subst; reflexivity. Qed.
-
-    Print z.
-    (* z =
-fun (r : Rank) (batch : Shape r) (pos n_heads d_model d_head : ShapeType) (n_ctx : N) (use_split_qkv_input : with_default "use_split_qkv_input" false)
-  (A : Type) (sqrtA : has_sqrt A) (coerZ : has_coer Z A) (addA : has_add A) (zeroA : has_zero A) (mulA : has_mul A) (divA : has_div A)
-  (expA : has_exp A) (defaultA : pointed A) (W_Q W_K W_V : tensor [n_heads; d_model; d_head] A) (b_Q b_K b_V : tensor [n_heads; d_head] A) =>
-let IGNORE := coerZ (-1 * 10 ^ 5)%Z in
-let attn_scale := √(coer φ (d_head)) in
-let maybe_n_heads := fun b : bool => if b as b0 return (Shape (if b0 then 1%nat else 0%nat)) then [n_heads]%shape else []%shape in
-fun query_input key_input value_input : tensor (batch ::' pos ++' (maybe_n_heads use_split_qkv_input ::' d_model)) A =>
-let mask := to_bool (tril (ones [of_Z n_ctx; of_Z n_ctx])) in
-PArray.checkpoint
-  (map2'
-     (fun (v : tensor [pos; n_heads; d_head] A) (pattern : tensor [n_heads; pos; pos] A) =>
-      (fun '(tt, i1, i0, i) => ∑_(0≤key_pos<pos)v.[[key_pos; i0; i]] * pattern.[[i0; i1; key_pos]]) : tensor [pos; n_heads; d_head] A)
-     (v W_V b_V value_input) (pattern W_Q W_K b_Q b_K query_input key_input))
-     : forall (r : Rank) (batch : Shape r) (pos n_heads d_model d_head : ShapeType),
-       N ->
-       forall (use_split_qkv_input : with_default "use_split_qkv_input" false) (A : Type),
-       has_sqrt A ->
-       has_coer Z A ->
-       has_add A ->
-       has_zero A ->
-       has_mul A ->
-       has_div A ->
-       has_exp A ->
-       pointed A ->
-       tensor [n_heads; d_model; d_head] A ->
-       tensor [n_heads; d_model; d_head] A ->
-       tensor [n_heads; d_model; d_head] A ->
-       tensor [n_heads; d_head] A ->
-       tensor [n_heads; d_head] A ->
-       tensor [n_heads; d_head] A ->
-       tensor
-         (batch ::' pos ++'
-          ((fun b : bool => if b as b0 return (Shape (if b0 then 1%nat else 0%nat)) then [n_heads]%shape else []%shape) use_split_qkv_input ::' d_model))
-         A ->
-       tensor
-         (batch ::' pos ++'
-          ((fun b : bool => if b as b0 return (Shape (if b0 then 1%nat else 0%nat)) then [n_heads]%shape else []%shape) use_split_qkv_input ::' d_model))
-         A ->
-       tensor
-         (batch ::' pos ++'
-          ((fun b : bool => if b as b0 return (Shape (if b0 then 1%nat else 0%nat)) then [n_heads]%shape else []%shape) use_split_qkv_input ::' d_model))
-         A -> tensor (batch ::' pos ::' n_heads ::' d_head) A
-
-Arguments z {r}%nat_scope {batch}%shape_scope {pos n_heads d_model d_head}%uint63_scope {n_ctx}%N_scope {use_split_qkv_input}
-  {A}%type_scope {sqrtA coerZ addA zeroA mulA divA expA defaultA} (W_Q W_K W_V b_Q b_K b_V query_input key_input value_input)%tensor_scope
-  _
-     *)
 
     #[export] Instance z_Proper_dep {r batch pos n_heads d_model d_head n_ctx use_split_qkv_input}
       : Dependent.Proper
@@ -563,60 +428,6 @@ Arguments z {r}%nat_scope {batch}%shape_scope {pos n_heads d_model d_head}%uint6
       : Proper (Tensor.eqf ==> Tensor.eqf ==> Tensor.eqf ==> Tensor.eqf)
         (@z r batch pos n_heads d_model d_head n_ctx use_split_qkv_input A sqrtA coerZ addA zeroA mulA divA expA defaultA W_Q W_K W_V b_Q b_K b_V).
     Proof. apply z_Proper_dep; repeat intro; subst; reflexivity. Qed.
-    Print attn_out.
-    (* attn_out =
-fun (r : Rank) (batch : Shape r) (pos n_heads d_model d_head : ShapeType) (n_ctx : N) (use_split_qkv_input : with_default "use_split_qkv_input" false)
-  (A : Type) (sqrtA : has_sqrt A) (coerZ : has_coer Z A) (addA : has_add A) (zeroA : has_zero A) (mulA : has_mul A) (divA : has_div A)
-  (expA : has_exp A) (defaultA : pointed A) (W_Q W_K W_V W_O : tensor [n_heads; d_model; d_head] A) (b_Q b_K b_V : tensor [n_heads; d_head] A)
-  (b_O : tensor [d_model] A) =>
-let IGNORE := coerZ (-1 * 10 ^ 5)%Z in
-let attn_scale := √(coer φ (d_head)) in
-let maybe_n_heads := fun b : bool => if b as b0 return (Shape (if b0 then 1%nat else 0%nat)) then [n_heads]%shape else []%shape in
-fun query_input key_input value_input : tensor (batch ::' pos ++' (maybe_n_heads use_split_qkv_input ::' d_model)) A =>
-let mask := to_bool (tril (ones [of_Z n_ctx; of_Z n_ctx])) in
-let out :=
-  map'
-    (fun z : tensor [pos; n_heads; d_head] A =>
-     (fun '(tt, i0, i) => ∑_(0≤head_index<n_heads)∑_(0≤d_head1<d_model)z.[[i0; head_index; d_head1]] * W_O.[[head_index; d_head1; i]])
-     :
-     tensor [pos; d_model] A) (z W_Q W_K W_V b_Q b_K b_V query_input key_input value_input) in
-PArray.checkpoint (out + broadcast b_O)%core
-     : forall (r : Rank) (batch : Shape r) (pos n_heads d_model d_head : ShapeType),
-       N ->
-       forall (use_split_qkv_input : with_default "use_split_qkv_input" false) (A : Type),
-       has_sqrt A ->
-       has_coer Z A ->
-       has_add A ->
-       has_zero A ->
-       has_mul A ->
-       has_div A ->
-       has_exp A ->
-       pointed A ->
-       tensor [n_heads; d_model; d_head] A ->
-       tensor [n_heads; d_model; d_head] A ->
-       tensor [n_heads; d_model; d_head] A ->
-       tensor [n_heads; d_model; d_head] A ->
-       tensor [n_heads; d_head] A ->
-       tensor [n_heads; d_head] A ->
-       tensor [n_heads; d_head] A ->
-       tensor [d_model] A ->
-       tensor
-         (batch ::' pos ++'
-          ((fun b : bool => if b as b0 return (Shape (if b0 then 1%nat else 0%nat)) then [n_heads]%shape else []%shape) use_split_qkv_input ::' d_model))
-         A ->
-       tensor
-         (batch ::' pos ++'
-          ((fun b : bool => if b as b0 return (Shape (if b0 then 1%nat else 0%nat)) then [n_heads]%shape else []%shape) use_split_qkv_input ::' d_model))
-         A ->
-       tensor
-         (batch ::' pos ++'
-          ((fun b : bool => if b as b0 return (Shape (if b0 then 1%nat else 0%nat)) then [n_heads]%shape else []%shape) use_split_qkv_input ::' d_model))
-         A -> tensor (batch ::' pos ::' d_model) A
-
-Arguments attn_out {r}%nat_scope {batch}%shape_scope {pos n_heads d_model d_head}%uint63_scope {n_ctx}%N_scope {use_split_qkv_input}
-  {A}%type_scope {sqrtA coerZ addA zeroA mulA divA expA defaultA} (W_Q W_K W_V W_O b_Q b_K b_V b_O query_input key_input value_input)%tensor_scope
-  _
-     *)
 
     #[export] Instance attn_out_Proper_dep {r batch pos n_heads d_model d_head n_ctx use_split_qkv_input}
       : Dependent.Proper
@@ -653,24 +464,6 @@ Arguments attn_out {r}%nat_scope {batch}%shape_scope {pos n_heads d_model d_head
   Module TransformerBlock.
     Export TransformerBlock.
 
-    Print add_head_dimension.
-    (* add_head_dimension =
-fun (r : Rank) (batch : Shape r) (pos n_heads d_model : ShapeType) (use_split_qkv_input : with_default "use_split_qkv_input" false) =>
-let maybe_n_heads := fun b : bool => if b as b0 return (Shape (if b0 then 1%nat else 0%nat)) then [n_heads]%shape else []%shape in
-fun (A : Type) (resid_pre : tensor (batch ::' pos ++' [d_model]) A) =>
-if use_split_qkv_input as use_split_qkv_input0 return (tensor (batch ::' pos ++' (maybe_n_heads use_split_qkv_input0 ::' d_model)) A)
-then map' (fun resid_pre0 : tensor [d_model] A => repeat [n_heads] resid_pre0 : tensor [n_heads; d_model] A) resid_pre
-else resid_pre
-     : forall (r : Rank) (batch : Shape r) (pos n_heads d_model : ShapeType) (use_split_qkv_input : with_default "use_split_qkv_input" false) (A : Type),
-       tensor (batch ::' pos ++' [d_model]) A ->
-       tensor
-         (batch ::' pos ++'
-          ((fun b : bool => if b as b0 return (Shape (if b0 then 1%nat else 0%nat)) then [n_heads]%shape else []%shape) use_split_qkv_input ::' d_model))
-         A
-
-Arguments add_head_dimension {r}%nat_scope {batch}%shape_scope {pos n_heads d_model}%uint63_scope {use_split_qkv_input} {A}%type_scope
-  resid_pre%tensor_scope _
-     *)
     #[export] Instance add_head_dimension_Proper_dep {r batch pos n_heads d_model use_split_qkv_input}
       : Dependent.Proper
           (Tensor.eqfR ==> Tensor.eqfR)
@@ -700,76 +493,6 @@ Arguments add_head_dimension {r}%nat_scope {batch}%shape_scope {pos n_heads d_mo
       : Proper (Tensor.eqf ==> Tensor.eqf) (@value_input r batch pos n_heads d_model use_split_qkv_input A)
       := _.
 
-    Print ln1.
-    (* ln1 =
-fun (r : Rank) (batch : Shape r) (pos n_heads d_model : ShapeType) (use_split_qkv_input : with_default "use_split_qkv_input" false)
-  (normalization_type : with_default "normalization_type" (Some LN)) =>
-let maybe_n_heads := fun b : bool => if b as b0 return (Shape (if b0 then 1%nat else 0%nat)) then [n_heads]%shape else []%shape in
-let ln_s := (batch ::' pos ++' maybe_n_heads use_split_qkv_input)%shape in
-fun (A : Type) (zeroA : has_zero A) (coerZ : has_coer Z A) (addA : has_add A) (subA : has_sub A) (mulA : has_mul A) (divA : has_div A)
-  (sqrtA : has_sqrt A) (default : pointed A) (eps : A)
-  (ln1_w ln1_b : match normalization_type with
-                 | Some LN => tensor [d_model] A
-                 | None => with_default "()" I
-                 end) (t : tensor (ln_s ::' d_model) A) =>
-match
-  normalization_type as normalization_type0
-  return
-    (match normalization_type0 with
-     | Some LN => tensor [d_model] A
-     | None => with_default "()" I
-     end ->
-     match normalization_type0 with
-     | Some LN => tensor [d_model] A
-     | None => with_default "()" I
-     end -> tensor (ln_s ::' d_model) A -> tensor (ln_s ::' d_model) A)
-with
-| Some n =>
-    match
-      n as n0
-      return
-        (match n0 with
-         | LN => tensor [d_model] A
-         end -> match n0 with
-                | LN => tensor [d_model] A
-                end -> tensor (ln_s ::' d_model) A -> tensor (ln_s ::' d_model) A)
-    with
-    | LN => LayerNorm.forward eps
-    end
-| None => fun _ _ : match None with
-                    | Some LN => tensor [d_model] A
-                    | None => with_default "()" I
-                    end => PArray.checkpoint
-end ln1_w ln1_b t
-     : forall (r : Rank) (batch : Shape r) (pos n_heads d_model : ShapeType) (use_split_qkv_input : with_default "use_split_qkv_input" false)
-         (normalization_type : with_default "normalization_type" (Some LN)) (A : Type),
-       has_zero A ->
-       has_coer Z A ->
-       has_add A ->
-       has_sub A ->
-       has_mul A ->
-       has_div A ->
-       has_sqrt A ->
-       pointed A ->
-       A ->
-       match normalization_type with
-       | Some LN => tensor [d_model] A
-       | None => with_default "()" I
-       end ->
-       match normalization_type with
-       | Some LN => tensor [d_model] A
-       | None => with_default "()" I
-       end ->
-       tensor
-         (batch ::' pos ++'
-          (fun b : bool => if b as b0 return (Shape (if b0 then 1%nat else 0%nat)) then [n_heads]%shape else []%shape) use_split_qkv_input ::' d_model) A ->
-       tensor
-         (batch ::' pos ++'
-          (fun b : bool => if b as b0 return (Shape (if b0 then 1%nat else 0%nat)) then [n_heads]%shape else []%shape) use_split_qkv_input ::' d_model) A
-
-Arguments ln1 {r}%nat_scope {batch}%shape_scope {pos n_heads d_model}%uint63_scope {use_split_qkv_input normalization_type} {A}%type_scope
-  {zeroA coerZ addA subA mulA divA sqrtA default} eps ln1_w ln1_b t%tensor_scope _
-     *)
     #[export] Instance ln1_Proper_dep {r batch pos n_heads d_model use_split_qkv_input normalization_type}
       : Dependent.Proper
           (Dependent.idR
@@ -826,76 +549,6 @@ Arguments ln1 {r}%nat_scope {batch}%shape_scope {pos n_heads d_model}%uint63_sco
       : Proper (Tensor.eqf ==> Tensor.eqf) (@ln2 r batch pos n_heads d_model use_split_kqv_input normalization_type A zeroA coerZ addA subA mulA divA sqrtA default eps ln2_w ln2_b).
     Proof. apply ln2_Proper_dep; repeat intro; subst; break_innermost_match; reflexivity. Qed.
 
-
-    Print attn_only_out.
-    (* attn_only_out =
-fun (r : Rank) (batch : Shape r) (pos n_heads d_model d_head : ShapeType)
-  (n_ctx : N) (use_split_qkv_input : with_default "use_split_qkv_input" false)
-  (normalization_type : with_default "normalization_type" (Some LN)) =>
-let maybe_n_heads :=
-  fun b : bool =>
-  if b as b0 return (Shape (if b0 then 1%nat else 0%nat))
-  then [n_heads]%shape
-  else []%shape in
-let ln_s := (batch ::' pos ++' maybe_n_heads use_split_qkv_input)%shape in
-fun (A : Type) (zeroA : has_zero A) (coerZ : has_coer Z A)
-  (addA : has_add A) (subA : has_sub A) (mulA : has_mul A)
-  (divA : has_div A) (sqrtA : has_sqrt A) (expA : has_exp A)
-  (default : pointed A) (W_Q W_K W_V W_O : tensor [n_heads; d_model; d_head] A)
-  (b_Q b_K b_V : tensor [n_heads; d_head] A) (b_O : tensor [d_model] A)
-  (eps : A)
-  (ln1_w
-   ln1_b : match normalization_type with
-           | Some LN => tensor [d_model] A
-           | None => with_default "()" I
-           end) (resid_pre : tensor (batch ::' pos ++' [d_model]) A) =>
-let attn_out :=
-  Attention.attn_out W_Q W_K W_V W_O b_Q b_K b_V b_O
-    (ln1 eps ln1_w ln1_b (query_input resid_pre))
-    (ln1 eps ln1_w ln1_b (key_input resid_pre))
-    (ln1 eps ln1_w ln1_b (value_input resid_pre)) in
-(resid_pre + attn_out)%core
-     : forall (r : Rank) (batch : Shape r) (pos n_heads d_model d_head : ShapeType),
-       N ->
-       with_default "use_split_qkv_input" false ->
-       forall (normalization_type : with_default "normalization_type" (Some LN))
-         (A : Type),
-       has_zero A ->
-       has_coer Z A ->
-       has_add A ->
-       has_sub A ->
-       has_mul A ->
-       has_div A ->
-       has_sqrt A ->
-       has_exp A ->
-       pointed A ->
-       tensor [n_heads; d_model; d_head] A ->
-       tensor [n_heads; d_model; d_head] A ->
-       tensor [n_heads; d_model; d_head] A ->
-       tensor [n_heads; d_model; d_head] A ->
-       tensor [n_heads; d_head] A ->
-       tensor [n_heads; d_head] A ->
-       tensor [n_heads; d_head] A ->
-       tensor [d_model] A ->
-       A ->
-       match normalization_type with
-       | Some LN => tensor [d_model] A
-       | None => with_default "()" I
-       end ->
-       match normalization_type with
-       | Some LN => tensor [d_model] A
-       | None => with_default "()" I
-       end ->
-       tensor (batch ::' pos ++' [d_model]) A ->
-       tensor (batch ++' [pos; d_model]) A
-
-Arguments attn_only_out {r}%nat_scope {batch}%shape_scope
-  {pos n_heads d_model d_head}%uint63_scope {n_ctx}%N_scope
-  {use_split_qkv_input normalization_type} {A}%type_scope
-  {zeroA coerZ addA subA mulA divA sqrtA expA default}
-  (W_Q W_K W_V W_O b_Q b_K b_V b_O)%tensor_scope eps ln1_w
-  ln1_b resid_pre%tensor_scope _
-     *)
     #[export] Instance attn_only_out_Proper_dep {r batch pos n_heads d_model d_head n_ctx use_split_qkv_input normalization_type}
       : Dependent.Proper
           (Dependent.idR
@@ -938,66 +591,6 @@ Arguments attn_only_out {r}%nat_scope {batch}%shape_scope
       : Proper (Tensor.eqf ==> Tensor.eqf) (@attn_only_out r batch pos n_heads d_model d_head n_ctx use_split_kqv_input normalization_type A zeroA coerZ addA subA mulA divA sqrtA expA default W_Q W_K W_V W_O b_Q b_K b_V b_O eps ln1_w ln1_b).
     Proof. apply attn_only_out_Proper_dep; repeat intro; subst; break_innermost_match; reflexivity. Qed.
 
-    Print HookedTransformer.TransformerBlock.attn_masked_attn_scores.
-    (* HookedTransformer.TransformerBlock.attn_masked_attn_scores =
-fun (r : Rank) (batch : Shape r) (pos n_heads d_model d_head : ShapeType)
-  (n_ctx : N) (use_split_qkv_input : with_default "use_split_qkv_input" false)
-  (normalization_type : with_default "normalization_type" (Some LN)) =>
-let maybe_n_heads :=
-  fun b : bool =>
-  if b as b0 return (Shape (if b0 then 1%nat else 0%nat))
-  then [n_heads]%shape
-  else []%shape in
-let ln_s := (batch ::' pos ++' maybe_n_heads use_split_qkv_input)%shape in
-fun (A : Type) (zeroA : has_zero A) (coerZ : has_coer Z A)
-  (addA : has_add A) (subA : has_sub A) (mulA : has_mul A)
-  (divA : has_div A) (sqrtA : has_sqrt A) (default : pointed A)
-  (W_Q W_K : tensor [n_heads; d_model; d_head] A)
-  (b_Q b_K : tensor [n_heads; d_head] A) (eps : A)
-  (ln1_w
-   ln1_b : match normalization_type with
-           | Some LN => tensor [d_model] A
-           | None => with_default "()" I
-           end) (resid_pre : tensor (batch ::' pos ++' [d_model]) A) =>
-Attention.masked_attn_scores W_Q W_K b_Q b_K
-  (ln1 eps ln1_w ln1_b (query_input resid_pre))
-  (ln1 eps ln1_w ln1_b (key_input resid_pre))
-     : forall (r : Rank) (batch : Shape r) (pos n_heads d_model d_head : ShapeType),
-       N ->
-       with_default "use_split_qkv_input" false ->
-       forall (normalization_type : with_default "normalization_type" (Some LN))
-         (A : Type),
-       has_zero A ->
-       has_coer Z A ->
-       has_add A ->
-       has_sub A ->
-       has_mul A ->
-       has_div A ->
-       has_sqrt A ->
-       pointed A ->
-       tensor [n_heads; d_model; d_head] A ->
-       tensor [n_heads; d_model; d_head] A ->
-       tensor [n_heads; d_head] A ->
-       tensor [n_heads; d_head] A ->
-       A ->
-       match normalization_type with
-       | Some LN => tensor [d_model] A
-       | None => with_default "()" I
-       end ->
-       match normalization_type with
-       | Some LN => tensor [d_model] A
-       | None => with_default "()" I
-       end ->
-       tensor (batch ::' pos ++' [d_model]) A ->
-       tensor (batch ::' n_heads ::' pos ::' pos) A
-
-Arguments HookedTransformer.TransformerBlock.attn_masked_attn_scores
-  {r}%nat_scope {batch}%shape_scope {pos n_heads d_model d_head}%uint63_scope
-  {n_ctx}%N_scope {use_split_qkv_input normalization_type}
-  {A}%type_scope {zeroA coerZ addA subA mulA divA sqrtA default}
-  (W_Q W_K b_Q b_K)%tensor_scope eps ln1_w ln1_b resid_pre%tensor_scope
-  _
-     *)
     #[export] Instance attn_masked_attn_scores_Proper_dep {r batch pos n_heads d_model d_head n_ctx use_split_qkv_input normalization_type}
       : Dependent.Proper
           (Dependent.idR
@@ -1034,28 +627,50 @@ Arguments HookedTransformer.TransformerBlock.attn_masked_attn_scores
     #[export] Instance attn_masked_attn_scores_Proper {r batch pos n_heads d_model d_head n_ctx use_split_kqv_input normalization_type A zeroA coerZ addA subA mulA divA sqrtA default W_Q W_K b_Q b_K eps ln1_w ln1_b}
       : Proper (Tensor.eqf ==> Tensor.eqf) (@HookedTransformer.TransformerBlock.attn_masked_attn_scores r batch pos n_heads d_model d_head n_ctx use_split_kqv_input normalization_type A zeroA coerZ addA subA mulA divA sqrtA default W_Q W_K b_Q b_K eps ln1_w ln1_b).
     Proof. apply attn_masked_attn_scores_Proper_dep; repeat intro; subst; break_innermost_match; reflexivity. Qed.
+
+    #[export] Instance attn_pattern_Proper_dep {r batch pos n_heads d_model d_head n_ctx use_split_qkv_input normalization_type}
+      : Dependent.Proper
+          (Dependent.idR
+             ==> (Dependent.const eq ==> Dependent.idR)
+             ==> (Dependent.idR ==> Dependent.idR ==> Dependent.idR)
+             ==> (Dependent.idR ==> Dependent.idR ==> Dependent.idR)
+             ==> (Dependent.idR ==> Dependent.idR ==> Dependent.idR)
+             ==> (Dependent.idR ==> Dependent.idR ==> Dependent.idR)
+             ==> (Dependent.idR ==> Dependent.idR)
+             ==> (Dependent.idR ==> Dependent.idR)
+             ==> Dependent.idR
+             ==> Tensor.eqfR
+             ==> Tensor.eqfR
+             ==> Tensor.eqfR
+             ==> Tensor.eqfR
+             ==> Dependent.idR
+             ==> match normalization_type return Dependent.relation (fun A => match normalization_type with Some LN => _ | None => _ end) with
+             | Some LN => Tensor.eqfR (s:=[d_model])
+             | None => Dependent.const eq
+             end
+             ==> match normalization_type return Dependent.relation (fun A => match normalization_type with Some LN => _ | None => _ end) with
+             | Some LN => Tensor.eqfR (s:=[d_model])
+             | None => Dependent.const eq
+             end
+             ==> Tensor.eqfR
+             ==> Tensor.eqfR)
+          (@HookedTransformer.TransformerBlock.attn_pattern r batch pos n_heads d_model d_head n_ctx use_split_qkv_input normalization_type).
+    Proof.
+      cbv [HookedTransformer.TransformerBlock.attn_pattern]; t.
+      all: apply Attention.pattern_Proper_dep; t.
+      all: apply ln1_Proper_dep; t.
+      all: first [ apply query_input_Proper_dep | apply key_input_Proper_dep ]; t.
+    Qed.
+
+    #[export] Instance attn_pattern_Proper {r batch pos n_heads d_model d_head n_ctx use_split_kqv_input normalization_type A zeroA coerZ addA subA mulA divA sqrtA expA default W_Q W_K b_Q b_K eps ln1_w ln1_b}
+      : Proper (Tensor.eqf ==> Tensor.eqf) (@HookedTransformer.TransformerBlock.attn_pattern r batch pos n_heads d_model d_head n_ctx use_split_kqv_input normalization_type A zeroA coerZ addA subA mulA divA sqrtA expA default W_Q W_K b_Q b_K eps ln1_w ln1_b).
+    Proof. apply attn_pattern_Proper_dep; repeat intro; subst; break_innermost_match; reflexivity. Qed.
   End TransformerBlock.
   Export (hints) TransformerBlock.
 
   Module HookedTransformer.
     Export HookedTransformer.
 
-    Print embed.
-    (* embed =
-fun (d_vocab d_model : ShapeType) (r : Rank) (batch : Shape r) (pos : ShapeType) =>
-let s := (batch ::' pos)%shape in
-let resid_shape := (s ::' d_model)%shape in
-fun (A : Type) (W_E : tensor [d_vocab; d_model] A) (tokens : tensor s IndexType) =>
-Embed.forward W_E tokens
-     : forall (d_vocab d_model : ShapeType) (r : Rank)
-         (batch : Shape r) (pos : ShapeType) (A : Type),
-       tensor [d_vocab; d_model] A ->
-       tensor (batch ::' pos) IndexType -> tensor (batch ::' pos ::' d_model) A
-
-Arguments embed {d_vocab d_model}%uint63_scope {r}%nat_scope
-  {batch}%shape_scope {pos}%uint63_scope {A}%type_scope
-  (W_E tokens)%tensor_scope _
-*)
     #[export] Instance embed_Proper_dep {d_vocab d_model r batch pos}
       : Dependent.Proper
           (Tensor.eqfR ==> Dependent.const Tensor.eqf ==> Tensor.eqfR)
@@ -1064,23 +679,7 @@ Arguments embed {d_vocab d_model}%uint63_scope {r}%nat_scope
     #[export] Instance embed_Proper {d_vocab d_model r batch pos A W_E}
       : Proper (Tensor.eqf ==> Tensor.eqf) (@embed d_vocab d_model r batch pos A W_E)
       := _.
-    Print pos_embed.
-    (* pos_embed =
-fun (d_model : ShapeType) (n_ctx : N) (r : Rank) (batch : Shape r)
-  (pos : ShapeType) =>
-let s := (batch ::' pos)%shape in
-let resid_shape := (s ::' d_model)%shape in
-fun (A : Type) (W_pos : tensor [of_Z n_ctx; d_model] A)
-  (tokens : tensor s IndexType) => PosEmbed.forward W_pos tokens
-     : forall (d_model : ShapeType) (n_ctx : N) (r : Rank)
-         (batch : Shape r) (pos : ShapeType) (A : Type),
-       tensor [of_Z n_ctx; d_model] A ->
-       tensor (batch ::' pos) IndexType -> tensor (batch ::' pos ::' d_model) A
 
-Arguments pos_embed {d_model}%uint63_scope {n_ctx}%N_scope
-  {r}%nat_scope {batch}%shape_scope {pos}%uint63_scope
-  {A}%type_scope (W_pos tokens)%tensor_scope _
-     *)
     #[export] Instance pos_embed_Proper_dep {d_model n_ctx r batch pos}
       : Dependent.Proper
           (Tensor.eqfR ==> Dependent.const Tensor.eqf ==> Tensor.eqfR)
@@ -1090,32 +689,6 @@ Arguments pos_embed {d_model}%uint63_scope {n_ctx}%N_scope
       : Proper (Tensor.eqf ==> Tensor.eqf) (@pos_embed d_model n_ctx r batch pos A W_pos)
       := _.
 
-    Print resid_postembed.
-    (* resid_postembed =
-fun (d_vocab d_model : ShapeType) (n_ctx : N) (r : Rank)
-  (batch : Shape r) (pos : ShapeType) =>
-let s := (batch ::' pos)%shape in
-let resid_shape := (s ::' d_model)%shape in
-fun (A : Type) (addA : has_add A) (default : pointed A)
-  (W_E : tensor [d_vocab; d_model] A) (W_pos : tensor [of_Z n_ctx; d_model] A)
-  (tokens : tensor s IndexType) =>
-let embed := embed W_E tokens in
-let pos_embed := pos_embed W_pos tokens in
-PArray.checkpoint (embed + pos_embed)%core
-     : forall (d_vocab d_model : ShapeType) (n_ctx : N)
-         (r : Rank) (batch : Shape r) (pos : ShapeType)
-         (A : Type),
-       has_add A ->
-       pointed A ->
-       tensor [d_vocab; d_model] A ->
-       tensor [of_Z n_ctx; d_model] A ->
-       tensor (batch ::' pos) IndexType -> tensor (batch ::' pos ::' d_model) A
-
-Arguments resid_postembed {d_vocab d_model}%uint63_scope
-  {n_ctx}%N_scope {r}%nat_scope {batch}%shape_scope {pos}%uint63_scope
-  {A}%type_scope {addA default} (W_E W_pos tokens)%tensor_scope
-  _
-     *)
     #[export] Instance resid_postembed_Proper_dep {d_vocab d_model n_ctx r batch pos}
       : Dependent.Proper
           ((Dependent.idR ==> Dependent.idR ==> Dependent.idR)
@@ -1129,76 +702,7 @@ Arguments resid_postembed {d_vocab d_model}%uint63_scope
       : Proper (Tensor.eqf ==> Tensor.eqf) (@resid_postembed d_vocab d_model n_ctx r batch pos A addA default W_E W_pos).
     Proof. apply resid_postembed_Proper_dep; repeat intro; subst; reflexivity. Qed.
 
-    Print blocks.
-    (* blocks =
-fun (n_heads d_model d_head : ShapeType) (n_ctx : N) (r : Rank)
-  (batch : Shape r) (pos : ShapeType) =>
-let s := (batch ::' pos)%shape in
-let resid_shape := (s ::' d_model)%shape in
-fun (A : Type) (zeroA : has_zero A) (coerZ : has_coer Z A)
-  (addA : has_add A) (subA : has_sub A) (mulA : has_mul A)
-  (divA : has_div A) (sqrtA : has_sqrt A) (expA : has_exp A)
-  (default : pointed A)
-  (normalization_type : with_default "normalization_type" (Some LN))
-  (eps : A)
-  (blocks_params : list
-                     (tensor [n_heads; d_model; d_head] A *
-                      tensor [n_heads; d_model; d_head] A *
-                      tensor [n_heads; d_model; d_head] A *
-                      tensor [n_heads; d_model; d_head] A *
-                      tensor [n_heads; d_head] A * tensor [n_heads; d_head] A *
-                      tensor [n_heads; d_head] A * tensor [d_model] A *
-                      match normalization_type with
-                      | Some LN => tensor [d_model] A
-                      | None => with_default "()" I
-                      end *
-                      match normalization_type with
-                      | Some LN => tensor [d_model] A
-                      | None => with_default "()" I
-                      end)) =>
-List.map
-  (fun '(W_Q, W_K, W_V, W_O, b_Q, b_K, b_V, b_O, ln1_w, ln1_b) =>
-   TransformerBlock.attn_only_out W_Q W_K W_V W_O b_Q b_K b_V b_O eps ln1_w ln1_b)
-  blocks_params
-     : forall n_heads d_model d_head : ShapeType,
-       N ->
-       forall (r : Rank) (batch : Shape r) (pos : ShapeType) (A : Type),
-       has_zero A ->
-       has_coer Z A ->
-       has_add A ->
-       has_sub A ->
-       has_mul A ->
-       has_div A ->
-       has_sqrt A ->
-       has_exp A ->
-       pointed A ->
-       forall normalization_type : with_default "normalization_type" (Some LN),
-       A ->
-       list
-         (tensor [n_heads; d_model; d_head] A * tensor [n_heads; d_model; d_head] A *
-          tensor [n_heads; d_model; d_head] A * tensor [n_heads; d_model; d_head] A *
-          tensor [n_heads; d_head] A * tensor [n_heads; d_head] A *
-          tensor [n_heads; d_head] A * tensor [d_model] A *
-          match normalization_type with
-          | Some LN => tensor [d_model] A
-          | None => with_default "()" I
-          end *
-          match normalization_type with
-          | Some LN => tensor [d_model] A
-          | None => with_default "()" I
-          end) ->
-       list
-         (tensor (batch ::' pos ::' d_model) A ->
-          tensor (batch ::' pos ::' d_model) A)
-
-Arguments blocks {n_heads d_model d_head}%uint63_scope
-  {n_ctx}%N_scope {r}%nat_scope {batch}%shape_scope {pos}%uint63_scope
-  {A}%type_scope
-  {zeroA coerZ addA subA mulA divA sqrtA expA default normalization_type}
-  eps blocks_params%list_scope
-     *)
-
-    #[export] Instance blocks_Proper_dep {n_heads d_model d_head n_ctx r batch pos normalization_type}
+    #[export] Polymorphic Instance blocks_Proper_dep {n_heads d_model d_head n_ctx r batch pos normalization_type}
       : Dependent.Proper
           (Dependent.idR
              ==> (Dependent.const eq ==> Dependent.idR)
@@ -1233,86 +737,10 @@ Arguments blocks {n_heads d_model d_head}%uint63_scope
       apply TransformerBlock.attn_only_out_Proper_dep; t.
     Qed.
 
-    #[export] Instance blocks_Proper {n_heads d_model d_head n_ctx r batch pos normalization_type A zeroA coerZ addA subA mulA divA sqrtA expA default eps blocks_params}
+    #[export] Polymorphic Instance blocks_Proper {n_heads d_model d_head n_ctx r batch pos normalization_type A zeroA coerZ addA subA mulA divA sqrtA expA default eps blocks_params}
       : Proper (List.Forall2 (Tensor.eqf ==> Tensor.eqf))%signature (@blocks n_heads d_model d_head n_ctx r batch pos normalization_type A zeroA coerZ addA subA mulA divA sqrtA expA default eps blocks_params).
     Proof. apply blocks_Proper_dep; repeat intro; subst; break_innermost_match; reflexivity. Qed.
 
-    Print ln_final.
-    (* ln_final =
-fun (d_model : ShapeType) (r : Rank) (batch : Shape r) (pos : ShapeType) =>
-let s := (batch ::' pos)%shape in
-let resid_shape := (s ::' d_model)%shape in
-fun (normalization_type : with_default "normalization_type" (Some LN))
-  (A : Type) (zeroA : has_zero A) (coerZ : has_coer Z A)
-  (addA : has_add A) (subA : has_sub A) (mulA : has_mul A)
-  (divA : has_div A) (sqrtA : has_sqrt A) (default : pointed A)
-  (eps : A)
-  (ln_final_w
-   ln_final_b : match normalization_type with
-                | Some LN => tensor [d_model] A
-                | None => with_default "()" I
-                end) (resid : tensor resid_shape A) =>
-match
-  normalization_type as normalization_type0
-  return
-    (match normalization_type0 with
-     | Some LN => tensor [d_model] A
-     | None => with_default "()" I
-     end ->
-     match normalization_type0 with
-     | Some LN => tensor [d_model] A
-     | None => with_default "()" I
-     end -> tensor (s ::' d_model) A -> tensor (s ::' d_model) A)
-with
-| Some n =>
-    match
-      n as n0
-      return
-        (match n0 with
-         | LN => tensor [d_model] A
-         end ->
-         match n0 with
-         | LN => tensor [d_model] A
-         end -> tensor (s ::' d_model) A -> tensor (s ::' d_model) A)
-    with
-    | LN => LayerNorm.forward eps
-    end
-| None =>
-    fun
-      (_
-       _ : match None with
-           | Some LN => tensor [d_model] A
-           | None => with_default "()" I
-           end) (t : tensor (s ::' d_model) A) => t
-end ln_final_w ln_final_b resid
-     : forall (d_model : ShapeType) (r : Rank) (batch : Shape r)
-         (pos : ShapeType)
-         (normalization_type : with_default "normalization_type" (Some LN))
-         (A : Type),
-       has_zero A ->
-       has_coer Z A ->
-       has_add A ->
-       has_sub A ->
-       has_mul A ->
-       has_div A ->
-       has_sqrt A ->
-       pointed A ->
-       A ->
-       match normalization_type with
-       | Some LN => tensor [d_model] A
-       | None => with_default "()" I
-       end ->
-       match normalization_type with
-       | Some LN => tensor [d_model] A
-       | None => with_default "()" I
-       end ->
-       tensor (batch ::' pos ::' d_model) A -> tensor (batch ::' pos ::' d_model) A
-
-Arguments ln_final {d_model}%uint63_scope {r}%nat_scope
-  {batch}%shape_scope {pos}%uint63_scope {normalization_type}
-  {A}%type_scope {zeroA coerZ addA subA mulA divA sqrtA default}
-  eps ln_final_w ln_final_b resid%tensor_scope _
-     *)
     #[export] Instance ln_final_Proper_dep {d_model r batch pos normalization_type}
       : Dependent.Proper
           (Dependent.idR
@@ -1381,67 +809,360 @@ Arguments unembed {d_vocab_out d_model}%uint63_scope {r}%nat_scope
       : Proper (Tensor.eqf ==> Tensor.eqf) (@unembed d_vocab_out d_model r batch pos A zeroA addA mulA W_U b_U)
       := _.
 
-    Print blocks_cps.
-
-    #[export] Instance blocks_cps_Proper {A zeroA coerZ addA subA mulA divA sqrtA expA default n_heads d_model d_head n_ctx normalization_type eps blocks_params r batch pos T R}
-      : Proper (eq ==> Tensor.eqf ==> (Tensor.eqf ==> R) ==> R) (@blocks_cps A zeroA coerZ addA subA mulA divA sqrtA expA default n_heads d_model d_head n_ctx normalization_type eps blocks_params r batch pos T).
+    #[export] Instance blocks_cps_Proper_dep {n_heads d_model d_head n_ctx r batch pos normalization_type}
+      : Dependent.Proper
+                           (Dependent.idR
+             ==> (Dependent.const eq ==> Dependent.idR)
+             ==> (Dependent.idR ==> Dependent.idR ==> Dependent.idR)
+             ==> (Dependent.idR ==> Dependent.idR ==> Dependent.idR)
+             ==> (Dependent.idR ==> Dependent.idR ==> Dependent.idR)
+             ==> (Dependent.idR ==> Dependent.idR ==> Dependent.idR)
+             ==> (Dependent.idR ==> Dependent.idR)
+             ==> (Dependent.idR ==> Dependent.idR)
+             ==> Dependent.idR
+             ==> Dependent.idR
+             ==> List.Forall2 ∘ (Tensor.eqfR * Tensor.eqfR
+                                 * Tensor.eqfR * Tensor.eqfR
+                                 * Tensor.eqfR * Tensor.eqfR
+                                 * Tensor.eqfR * Tensor.eqfR
+                                 * match normalization_type return Dependent.relation (fun A => match normalization_type with Some LN => _ | None => _ end) with
+                                   | Some LN => Tensor.eqfR (s:=[d_model])
+                                   | None => Dependent.const eq
+                                   end
+                                 * match normalization_type return Dependent.relation (fun A => match normalization_type with Some LN => _ | None => _ end) with
+                                   | Some LN => Tensor.eqfR (s:=[d_model])
+                                   | None => Dependent.const eq
+                                   end)
+             ==> Dependent.forall_relation
+             (Dependent.const2 (@eq nat (* strip dependency of with_default *))
+                ==> Dependent.lift2_1 Tensor.eqfR
+                ==> (Dependent.lift2_1 Tensor.eqfR ==> Dependent.lift2_2 Dependent.idR)
+                ==> Dependent.lift2_2 Dependent.idR))
+                           (@blocks_cps n_heads d_model d_head n_ctx r batch pos normalization_type).
     Proof.
-      cbv [blocks_cps with_default]; intros n ? <-; revert n.
-      let blocks := lazymatch goal with |- context[fold_right _ _ (List.firstn _ ?ls)] => ls end in
-      pose proof (blocks_Proper : List.Forall2 _ blocks blocks) as H.
-      induction blocks as [|?? IH], n; inversion H; clear H; subst; cbn [fold_right List.firstn]; [ now t .. | ].
-      repeat intro.
-      apply IH; clear IH; t; assumption.
+      cbv [Dependent.Proper Dependent.respectful blocks_cps with_default Dependent.forall_relation Dependent.respectful2]; clear.
+      repeat first [ lazymatch goal with H : Forall2 _ _ _ |- _ => fail 1 end | intro ].
+      let H := match goal with H : Forall2 _ _ _ |- _ => H end in
+      induction H; cbn [fold_right List.map].
+      all: intros; subst.
+      all: let n := lazymatch goal with |- context[firstn ?n] => n end in
+           is_var n; destruct n; cbn [fold_right firstn].
+      all: eauto.
+      all: [ > ].
+      cbv [blocks] in *; cbn [List.map firstn fold_right] in *.
+      let IH := multimatch goal with H : _ |- _ => H end in
+      apply IH; clear IH; repeat intro; eauto; [].
+      break_innermost_match.
+      apply Tensor.PArray.checkpoint_Proper_dep; try assumption; [].
+      apply TransformerBlock.attn_only_out_Proper_dep; t.
     Qed.
 
-    #[export] Instance logits_Proper {A zeroA coerZ addA subA mulA divA sqrtA expA default d_vocab d_vocab_out n_heads d_model d_head n_ctx normalization_type eps W_E W_pos blocks_params ln_final_w ln_final_b W_U b_U r batch pos}
-      : Proper (Tensor.eqf ==> Tensor.eqf) (@logits A zeroA coerZ addA subA mulA divA sqrtA expA default d_vocab d_vocab_out n_heads d_model d_head n_ctx normalization_type eps W_E W_pos blocks_params ln_final_w ln_final_b W_U b_U r batch pos).
+    #[export] Instance blocks_cps_Proper {n_heads d_model d_head n_ctx r batch pos normalization_type A zeroA coerZ addA subA mulA divA sqrtA expA default eps blocks_params T R}
+      : Proper (eq ==> Tensor.eqf ==> (Tensor.eqf ==> R) ==> R)
+          (@blocks_cps n_heads d_model d_head n_ctx r batch pos normalization_type A zeroA coerZ addA subA mulA divA sqrtA expA default eps blocks_params T).
+    Proof. apply blocks_cps_Proper_dep; repeat intro; subst; break_innermost_match; reflexivity. Qed.
+
+    #[export] Instance logits_Proper_dep {d_vocab d_vocab_out n_heads d_model d_head n_ctx r batch pos normalization_type}
+      : Dependent.Proper
+          (Dependent.idR
+             ==> (Dependent.const eq ==> Dependent.idR)
+             ==> (Dependent.idR ==> Dependent.idR ==> Dependent.idR)
+             ==> (Dependent.idR ==> Dependent.idR ==> Dependent.idR)
+             ==> (Dependent.idR ==> Dependent.idR ==> Dependent.idR)
+             ==> (Dependent.idR ==> Dependent.idR ==> Dependent.idR)
+             ==> (Dependent.idR ==> Dependent.idR)
+             ==> (Dependent.idR ==> Dependent.idR)
+             ==> Dependent.idR
+             ==> Dependent.idR
+             ==> Tensor.eqfR
+             ==> Tensor.eqfR
+             ==> List.Forall2 ∘ (Tensor.eqfR * Tensor.eqfR
+                                 * Tensor.eqfR * Tensor.eqfR
+                                 * Tensor.eqfR * Tensor.eqfR
+                                 * Tensor.eqfR * Tensor.eqfR
+                                 * match normalization_type return Dependent.relation (fun A => match normalization_type with Some LN => _ | None => _ end) with
+                                   | Some LN => Tensor.eqfR (s:=[d_model])
+                                   | None => Dependent.const eq
+                                   end
+                                 * match normalization_type return Dependent.relation (fun A => match normalization_type with Some LN => _ | None => _ end) with
+                                   | Some LN => Tensor.eqfR (s:=[d_model])
+                                   | None => Dependent.const eq
+                                   end)
+             ==> match normalization_type return Dependent.relation (fun A => match normalization_type with Some LN => _ | None => _ end) with
+             | Some LN => Tensor.eqfR (s:=[d_model])
+             | None => Dependent.const eq
+             end
+             ==> match normalization_type return Dependent.relation (fun A => match normalization_type with Some LN => _ | None => _ end) with
+             | Some LN => Tensor.eqfR (s:=[d_model])
+             | None => Dependent.const eq
+             end
+             ==> Tensor.eqfR
+             ==> Tensor.eqfR
+             ==> Dependent.const Tensor.eqf
+             ==> Tensor.eqfR)
+          (@logits d_vocab d_vocab_out n_heads d_model d_head n_ctx r batch pos normalization_type).
     Proof.
-      cbv [logits]; t.
-      refine (blocks_cps_Proper (R:=Tensor.eqf) _ _ _ _); t.
-      all: first [ apply resid_postembed_Proper | apply embed_Proper | apply pos_embed_Proper | apply unembed_Proper ]; t.
-      apply ln_final_Proper; t.
+      cbv [logits]; t; [].
+      lazymatch goal with
+      | [ |- ?R (?f ?i) (?g ?i) ]
+        => revert i; change ((fun F G => forall i, R (F i) (G i)) f g)
+      end.
+      eapply blocks_cps_Proper_dep; [ eassumption | .. ].
+      all: repeat intro; subst; t.
+      all: try now eapply Forall2_length, blocks_Proper_dep; eassumption.
+      all: first [ apply resid_postembed_Proper_dep | apply embed_Proper_dep | apply pos_embed_Proper_dep | apply ln_final_Proper_dep | apply unembed_Proper_dep ]; t.
     Qed.
 
-    #[export] Instance forward_Proper {A zeroA coerZ addA subA mulA divA sqrtA expA default d_vocab d_vocab_out n_heads d_model d_head n_ctx normalization_type eps W_E W_pos blocks_params ln_final_w ln_final_b W_U b_U r batch pos}
-      : Proper (Tensor.eqf ==> Tensor.eqf) (@forward A zeroA coerZ addA subA mulA divA sqrtA expA default d_vocab d_vocab_out n_heads d_model d_head n_ctx normalization_type eps W_E W_pos blocks_params ln_final_w ln_final_b W_U b_U r batch pos)
+    #[export] Instance logits_Proper {d_vocab d_vocab_out n_heads d_model d_head n_ctx r batch pos normalization_type A zeroA coerZ addA subA mulA divA sqrtA expA default eps W_E W_pos blocks_params ln_final_w ln_final_b W_U b_U}
+      : Proper (Tensor.eqf ==> Tensor.eqf)
+          (@logits d_vocab d_vocab_out n_heads d_model d_head n_ctx r batch pos normalization_type A zeroA coerZ addA subA mulA divA sqrtA expA default eps W_E W_pos blocks_params ln_final_w ln_final_b W_U b_U).
+    Proof. apply logits_Proper_dep; repeat intro; subst; break_innermost_match; reflexivity. Qed.
+
+    #[export] Instance forward_Proper_dep {d_vocab d_vocab_out n_heads d_model d_head n_ctx r batch pos normalization_type}
+      : Dependent.Proper
+          (Dependent.idR
+             ==> (Dependent.const eq ==> Dependent.idR)
+             ==> (Dependent.idR ==> Dependent.idR ==> Dependent.idR)
+             ==> (Dependent.idR ==> Dependent.idR ==> Dependent.idR)
+             ==> (Dependent.idR ==> Dependent.idR ==> Dependent.idR)
+             ==> (Dependent.idR ==> Dependent.idR ==> Dependent.idR)
+             ==> (Dependent.idR ==> Dependent.idR)
+             ==> (Dependent.idR ==> Dependent.idR)
+             ==> Dependent.idR
+             ==> Dependent.idR
+             ==> Tensor.eqfR
+             ==> Tensor.eqfR
+             ==> List.Forall2 ∘ (Tensor.eqfR * Tensor.eqfR
+                                 * Tensor.eqfR * Tensor.eqfR
+                                 * Tensor.eqfR * Tensor.eqfR
+                                 * Tensor.eqfR * Tensor.eqfR
+                                 * match normalization_type return Dependent.relation (fun A => match normalization_type with Some LN => _ | None => _ end) with
+                                   | Some LN => Tensor.eqfR (s:=[d_model])
+                                   | None => Dependent.const eq
+                                   end
+                                 * match normalization_type return Dependent.relation (fun A => match normalization_type with Some LN => _ | None => _ end) with
+                                   | Some LN => Tensor.eqfR (s:=[d_model])
+                                   | None => Dependent.const eq
+                                   end)
+             ==> match normalization_type return Dependent.relation (fun A => match normalization_type with Some LN => _ | None => _ end) with
+             | Some LN => Tensor.eqfR (s:=[d_model])
+             | None => Dependent.const eq
+             end
+             ==> match normalization_type return Dependent.relation (fun A => match normalization_type with Some LN => _ | None => _ end) with
+             | Some LN => Tensor.eqfR (s:=[d_model])
+             | None => Dependent.const eq
+             end
+             ==> Tensor.eqfR
+             ==> Tensor.eqfR
+             ==> Dependent.const Tensor.eqf
+             ==> Tensor.eqfR)
+          (@forward d_vocab d_vocab_out n_heads d_model d_head n_ctx r batch pos normalization_type)
       := _.
 
-    #[export] Instance blocks_attn_masked_attn_scores_Proper {A zeroA coerZ addA subA mulA divA sqrtA default n_heads d_model d_head n_ctx normalization_type eps blocks_params r batch pos}
-      : Proper (List.Forall2 (Tensor.eqf ==> Tensor.eqf))%signature (@HookedTransformer.HookedTransformer.blocks_attn_masked_attn_scores A zeroA coerZ addA subA mulA divA sqrtA default n_heads d_model d_head n_ctx normalization_type eps blocks_params r batch pos).
+    #[export] Instance forward_Proper {d_vocab d_vocab_out n_heads d_model d_head n_ctx r batch pos normalization_type A zeroA coerZ addA subA mulA divA sqrtA expA default eps W_E W_pos blocks_params ln_final_w ln_final_b W_U b_U}
+      : Proper (Tensor.eqf ==> Tensor.eqf)
+          (@forward d_vocab d_vocab_out n_heads d_model d_head n_ctx r batch pos normalization_type A zeroA coerZ addA subA mulA divA sqrtA expA default eps W_E W_pos blocks_params ln_final_w ln_final_b W_U b_U)
+      := _.
+
+    #[export] Instance blocks_attn_masked_attn_scores_Proper_dep {n_heads d_model d_head n_ctx r batch pos normalization_type}
+      : Dependent.Proper
+          (Dependent.idR
+             ==> (Dependent.const eq ==> Dependent.idR)
+             ==> (Dependent.idR ==> Dependent.idR ==> Dependent.idR)
+             ==> (Dependent.idR ==> Dependent.idR ==> Dependent.idR)
+             ==> (Dependent.idR ==> Dependent.idR ==> Dependent.idR)
+             ==> (Dependent.idR ==> Dependent.idR ==> Dependent.idR)
+             ==> (Dependent.idR ==> Dependent.idR)
+             ==> Dependent.idR
+             ==> Dependent.idR
+             ==> List.Forall2 ∘ (Tensor.eqfR * Tensor.eqfR
+                                 * Tensor.eqfR * Tensor.eqfR
+                                 * Tensor.eqfR * Tensor.eqfR
+                                 * Tensor.eqfR * Tensor.eqfR
+                                 * match normalization_type return Dependent.relation (fun A => match normalization_type with Some LN => _ | None => _ end) with
+                                   | Some LN => Tensor.eqfR (s:=[d_model])
+                                   | None => Dependent.const eq
+                                   end
+                                 * match normalization_type return Dependent.relation (fun A => match normalization_type with Some LN => _ | None => _ end) with
+                                   | Some LN => Tensor.eqfR (s:=[d_model])
+                                   | None => Dependent.const eq
+                                   end)
+             ==> List.Forall2 ∘ (Tensor.eqfR ==> Tensor.eqfR))
+          (@HookedTransformer.HookedTransformer.blocks_attn_masked_attn_scores n_heads d_model d_head n_ctx r batch pos normalization_type).
     Proof.
-      cbv [Proper HookedTransformer.HookedTransformer.blocks_attn_masked_attn_scores]; clear.
-      induction blocks_params as [|?? IH]; cbn [List.map]; constructor; auto; [].
+      cbv [Dependent.Proper HookedTransformer.HookedTransformer.blocks_attn_masked_attn_scores]; clear.
+      repeat first [ lazymatch goal with H : Forall2 _ _ _ |- _ => fail 1 end | intro ].
+      let H := match goal with H : Forall2 _ _ _ |- _ => H end in
+      induction H; cbn [List.map]; constructor; auto; [].
       destruct_head'_prod.
-      apply TransformerBlock.attn_masked_attn_scores_Proper.
+      apply TransformerBlock.attn_masked_attn_scores_Proper_dep; t.
     Qed.
 
-    #[export] Instance blocks_attn_pattern_Proper {A zeroA coerZ addA subA mulA divA sqrtA expA default n_heads d_model d_head n_ctx normalization_type eps blocks_params r batch pos}
-      : Proper (List.Forall2 (Tensor.eqf ==> Tensor.eqf))%signature (@HookedTransformer.HookedTransformer.blocks_attn_pattern A zeroA coerZ addA subA mulA divA sqrtA expA default n_heads d_model d_head n_ctx normalization_type eps blocks_params r batch pos).
+    #[export] Instance blocks_attn_masked_attn_scores_Proper {n_heads d_model d_head n_ctx r batch pos normalization_type A zeroA coerZ addA subA mulA divA sqrtA default eps blocks_params}
+      : Proper (List.Forall2 (Tensor.eqf ==> Tensor.eqf))%signature
+          (@HookedTransformer.HookedTransformer.blocks_attn_masked_attn_scores n_heads d_model d_head n_ctx r batch pos normalization_type A zeroA coerZ addA subA mulA divA sqrtA default eps blocks_params).
+    Proof. apply blocks_attn_masked_attn_scores_Proper_dep; repeat intro; subst; break_innermost_match; reflexivity. Qed.
+
+    #[export] Instance blocks_attn_pattern_Proper_dep {n_heads d_model d_head n_ctx r batch pos normalization_type}
+      : Dependent.Proper
+          (Dependent.idR
+             ==> (Dependent.const eq ==> Dependent.idR)
+             ==> (Dependent.idR ==> Dependent.idR ==> Dependent.idR)
+             ==> (Dependent.idR ==> Dependent.idR ==> Dependent.idR)
+             ==> (Dependent.idR ==> Dependent.idR ==> Dependent.idR)
+             ==> (Dependent.idR ==> Dependent.idR ==> Dependent.idR)
+             ==> (Dependent.idR ==> Dependent.idR)
+             ==> (Dependent.idR ==> Dependent.idR)
+             ==> Dependent.idR
+             ==> Dependent.idR
+             ==> List.Forall2 ∘ (Tensor.eqfR * Tensor.eqfR
+                                 * Tensor.eqfR * Tensor.eqfR
+                                 * Tensor.eqfR * Tensor.eqfR
+                                 * Tensor.eqfR * Tensor.eqfR
+                                 * match normalization_type return Dependent.relation (fun A => match normalization_type with Some LN => _ | None => _ end) with
+                                   | Some LN => Tensor.eqfR (s:=[d_model])
+                                   | None => Dependent.const eq
+                                   end
+                                 * match normalization_type return Dependent.relation (fun A => match normalization_type with Some LN => _ | None => _ end) with
+                                   | Some LN => Tensor.eqfR (s:=[d_model])
+                                   | None => Dependent.const eq
+                                   end)
+             ==> List.Forall2 ∘ (Tensor.eqfR ==> Tensor.eqfR))
+          (@HookedTransformer.HookedTransformer.blocks_attn_pattern n_heads d_model d_head n_ctx r batch pos normalization_type).
     Proof.
-      cbv [Proper HookedTransformer.HookedTransformer.blocks_attn_pattern]; clear.
-      induction blocks_params as [|?? IH]; cbn [List.map]; constructor; auto; [].
+      cbv [Dependent.Proper HookedTransformer.HookedTransformer.blocks_attn_pattern]; clear.
+      repeat first [ lazymatch goal with H : Forall2 _ _ _ |- _ => fail 1 end | intro ].
+      let H := match goal with H : Forall2 _ _ _ |- _ => H end in
+      induction H; cbn [List.map]; constructor; auto; [].
       destruct_head'_prod.
-      apply TransformerBlock.attn_pattern_Proper.
+      apply TransformerBlock.attn_pattern_Proper_dep; t.
     Qed.
 
-    #[export] Instance masked_attn_scores_Proper {A zeroA coerZ addA subA mulA divA sqrtA expA default d_vocab n_heads d_model d_head n_ctx normalization_type eps W_E W_pos blocks_params r batch pos}
-      : Proper (eq ==> Tensor.eqf ==> option_eq Tensor.eqf) (@HookedTransformer.HookedTransformer.masked_attn_scores A zeroA coerZ addA subA mulA divA sqrtA expA default d_vocab n_heads d_model d_head n_ctx normalization_type eps W_E W_pos blocks_params r batch pos).
+    #[export] Instance blocks_attn_pattern_Proper {n_heads d_model d_head n_ctx r batch pos normalization_type A zeroA coerZ addA subA mulA divA sqrtA expA default eps blocks_params}
+      : Proper (List.Forall2 (Tensor.eqf ==> Tensor.eqf))%signature
+          (@HookedTransformer.HookedTransformer.blocks_attn_pattern n_heads d_model d_head n_ctx r batch pos normalization_type A zeroA coerZ addA subA mulA divA sqrtA expA default eps blocks_params).
+    Proof. apply blocks_attn_pattern_Proper_dep; repeat intro; subst; break_innermost_match; reflexivity. Qed.
+
+    #[export] Instance masked_attn_scores_Proper_dep {d_vocab n_heads d_model d_head n_ctx r batch pos normalization_type}
+      : Dependent.Proper
+          (Dependent.idR
+             ==> (Dependent.const eq ==> Dependent.idR)
+             ==> (Dependent.idR ==> Dependent.idR ==> Dependent.idR)
+             ==> (Dependent.idR ==> Dependent.idR ==> Dependent.idR)
+             ==> (Dependent.idR ==> Dependent.idR ==> Dependent.idR)
+             ==> (Dependent.idR ==> Dependent.idR ==> Dependent.idR)
+             ==> (Dependent.idR ==> Dependent.idR)
+             ==> (Dependent.idR ==> Dependent.idR)
+             ==> Dependent.idR
+             ==> Dependent.idR
+             ==> Tensor.eqfR
+             ==> Tensor.eqfR
+             ==> List.Forall2 ∘ (Tensor.eqfR * Tensor.eqfR
+                                 * Tensor.eqfR * Tensor.eqfR
+                                 * Tensor.eqfR * Tensor.eqfR
+                                 * Tensor.eqfR * Tensor.eqfR
+                                 * match normalization_type return Dependent.relation (fun A => match normalization_type with Some LN => _ | None => _ end) with
+                                   | Some LN => Tensor.eqfR (s:=[d_model])
+                                   | None => Dependent.const eq
+                                   end
+                                 * match normalization_type return Dependent.relation (fun A => match normalization_type with Some LN => _ | None => _ end) with
+                                   | Some LN => Tensor.eqfR (s:=[d_model])
+                                   | None => Dependent.const eq
+                                   end)
+             ==> Dependent.const eq
+             ==> Dependent.const Tensor.eqf
+             ==> @option_eq ∘ Tensor.eqfR)
+          (@HookedTransformer.HookedTransformer.masked_attn_scores d_vocab n_heads d_model d_head n_ctx r batch pos normalization_type).
     Proof.
-      intros n ? <-.
-      cbv [HookedTransformer.HookedTransformer.masked_attn_scores]; t; try now constructor.
-      refine (blocks_cps_Proper (R:=Tensor.eqf) _ _ _ _); t.
-      apply resid_postembed_Proper; t.
+      cbv [HookedTransformer.HookedTransformer.masked_attn_scores option_eq]; t.
+      all: break_innermost_match_hyps; inversion_option; subst.
+      all: lazymatch goal with
+           | [ Hx : nth_error ?xs ?n = _, Hy : nth_error ?ys ?n = _ |- _ ]
+             => let H' := fresh in
+                unshelve
+                  (epose proof (List.nth_error_Proper_dep_Forall2
+                                  _ _ _
+                                  xs ys
+                                  (blocks_attn_masked_attn_scores_Proper_dep _ _ _ _ _ _ _ _ _ _ _ _ _ _ _ _)
+                                  n n eq_refl) as H';
+                   rewrite Hx, Hy in H'; cbv [option_eq] in H'; clear Hx Hy;
+                   try now exfalso);
+                shelve_unifiable; repeat intro; cbv beta; subst; try eassumption; eauto
+           end.
+      all: lazymatch goal with
+           | [ |- ?R (?f ?i) (?g ?i) ]
+             => revert i; change ((fun F G => forall i, R (F i) (G i)) f g)
+           end.
+      all: eapply blocks_cps_Proper_dep; [ eassumption | .. ].
+      all: repeat intro; subst; t.
+      all: try now eapply Forall2_length, blocks_Proper_dep; eassumption.
+      all: first [ apply resid_postembed_Proper_dep | apply embed_Proper_dep | apply pos_embed_Proper_dep | apply ln_final_Proper_dep | apply unembed_Proper_dep ]; t.
     Qed.
 
-    #[export] Instance attn_pattern_Proper {A zeroA coerZ addA subA mulA divA sqrtA expA default d_vocab n_heads d_model d_head n_ctx normalization_type eps W_E W_pos blocks_params r batch pos}
-      : Proper (eq ==> Tensor.eqf ==> option_eq Tensor.eqf) (@HookedTransformer.HookedTransformer.attn_pattern A zeroA coerZ addA subA mulA divA sqrtA expA default d_vocab n_heads d_model d_head n_ctx normalization_type eps W_E W_pos blocks_params r batch pos).
+    #[export] Instance masked_attn_scores_Proper {d_vocab n_heads d_model d_head n_ctx r batch pos normalization_type A zeroA coerZ addA subA mulA divA sqrtA expA default eps W_E W_pos blocks_params}
+      : Proper (eq ==> Tensor.eqf ==> option_eq Tensor.eqf)
+          (@HookedTransformer.HookedTransformer.masked_attn_scores d_vocab n_heads d_model d_head n_ctx r batch pos normalization_type A zeroA coerZ addA subA mulA divA sqrtA expA default eps W_E W_pos blocks_params).
+    Proof. apply masked_attn_scores_Proper_dep; repeat intro; subst; break_innermost_match; reflexivity. Qed.
+
+    #[export] Instance attn_pattern_Proper_dep {d_vocab n_heads d_model d_head n_ctx r batch pos normalization_type}
+      : Dependent.Proper
+          (Dependent.idR
+             ==> (Dependent.const eq ==> Dependent.idR)
+             ==> (Dependent.idR ==> Dependent.idR ==> Dependent.idR)
+             ==> (Dependent.idR ==> Dependent.idR ==> Dependent.idR)
+             ==> (Dependent.idR ==> Dependent.idR ==> Dependent.idR)
+             ==> (Dependent.idR ==> Dependent.idR ==> Dependent.idR)
+             ==> (Dependent.idR ==> Dependent.idR)
+             ==> (Dependent.idR ==> Dependent.idR)
+             ==> Dependent.idR
+             ==> Dependent.idR
+             ==> Tensor.eqfR
+             ==> Tensor.eqfR
+             ==> List.Forall2 ∘ (Tensor.eqfR * Tensor.eqfR
+                                 * Tensor.eqfR * Tensor.eqfR
+                                 * Tensor.eqfR * Tensor.eqfR
+                                 * Tensor.eqfR * Tensor.eqfR
+                                 * match normalization_type return Dependent.relation (fun A => match normalization_type with Some LN => _ | None => _ end) with
+                                   | Some LN => Tensor.eqfR (s:=[d_model])
+                                   | None => Dependent.const eq
+                                   end
+                                 * match normalization_type return Dependent.relation (fun A => match normalization_type with Some LN => _ | None => _ end) with
+                                   | Some LN => Tensor.eqfR (s:=[d_model])
+                                   | None => Dependent.const eq
+                                   end)
+             ==> Dependent.const eq
+             ==> Dependent.const Tensor.eqf
+             ==> @option_eq ∘ Tensor.eqfR)
+          (@HookedTransformer.HookedTransformer.attn_pattern d_vocab n_heads d_model d_head n_ctx r batch pos normalization_type).
     Proof.
-      intros n ? <-.
-      cbv [HookedTransformer.HookedTransformer.attn_pattern]; t; try now constructor.
-      refine (blocks_cps_Proper (R:=Tensor.eqf) _ _ _ _); t.
-      apply resid_postembed_Proper; t.
+      cbv [HookedTransformer.HookedTransformer.attn_pattern option_eq]; t.
+      all: break_innermost_match_hyps; inversion_option; subst.
+      all: lazymatch goal with
+           | [ Hx : nth_error ?xs ?n = _, Hy : nth_error ?ys ?n = _ |- _ ]
+             => let H' := fresh in
+                unshelve
+                  (epose proof (List.nth_error_Proper_dep_Forall2
+                                  _ _ _
+                                  xs ys
+                                  (blocks_attn_pattern_Proper_dep _ _ _ _ _ _ _ _ _ _ _ _ _ _ _ _ _)
+                                  n n eq_refl) as H';
+                   rewrite Hx, Hy in H'; cbv [option_eq] in H'; clear Hx Hy;
+                   try now exfalso);
+                shelve_unifiable; repeat intro; cbv beta; subst; try eassumption; eauto
+           end.
+      all: lazymatch goal with
+           | [ |- ?R (?f ?i) (?g ?i) ]
+             => revert i; change ((fun F G => forall i, R (F i) (G i)) f g)
+           end.
+      all: eapply blocks_cps_Proper_dep; [ eassumption | .. ].
+      all: repeat intro; subst; t.
+      all: first [ apply resid_postembed_Proper_dep | apply embed_Proper_dep | apply pos_embed_Proper_dep | apply ln_final_Proper_dep | apply unembed_Proper_dep ]; t.
     Qed.
+
+    #[export] Instance attn_pattern_Proper {d_vocab n_heads d_model d_head n_ctx r batch pos normalization_type A zeroA coerZ addA subA mulA divA sqrtA expA default eps W_E W_pos blocks_params}
+      : Proper (eq ==> Tensor.eqf ==> option_eq Tensor.eqf)
+          (@HookedTransformer.HookedTransformer.attn_pattern d_vocab n_heads d_model d_head n_ctx r batch pos normalization_type A zeroA coerZ addA subA mulA divA sqrtA expA default eps W_E W_pos blocks_params).
+    Proof. apply attn_pattern_Proper_dep; repeat intro; subst; break_innermost_match; reflexivity. Qed.
   End HookedTransformer.
   Export (hints) HookedTransformer.
 End HookedTransformer.
