theories/Util/List/Instances/NthError.v
@@ -1,14 +1,20 @@
 From Coq Require Import List Morphisms.
 From NeuralNetInterp.Util Require Import Option.
+From NeuralNetInterp.Util Require Morphisms.Dependent.
 Import ListNotations.
+Import Dependent.ProperNotations.
 #[local] Open Scope list_scope.
 
 Module List.
-  #[export] Instance nth_error_Proper_Forall2 {A R}
-  : Proper (Forall2 R ==> eq ==> option_eq R) (@nth_error A).
+  #[export] Instance nth_error_Proper_dep_Forall2
+  : Dependent.Proper (Forall2 ==> Dependent.const eq ==> @option_eq) (@nth_error).
   Proof.
-    intros ?? H n ? <-; revert n.
+    intros ?? HR ?? H n ? <-; revert n.
     now induction H, n; cbn.
   Qed.
+
+  #[export] Instance nth_error_Proper_Forall2 {A R}
+  : Proper (Forall2 R ==> eq ==> option_eq R) (@nth_error A).
+  Proof. apply nth_error_Proper_dep_Forall2. Qed.
 End List.
 Export (hints) List.
