theories/Util/Program/Basics/Dependent.v
@@ -1,4 +1,4 @@
-From Coq Require Import Program.Basics.
+From Coq Require Import Program.Basics Utf8.
 Declare Scope type_function_scope.
 Declare Scope type_function2_scope.
 Declare Scope type_function3_scope.
@@ -26,16 +26,23 @@ Notation "X -> Y" := (fun A : Type => X%type_function A -> Y%type_function A) : 
 Notation "X * Y" := (fun A : Type => prod (X%type_function A) (Y%type_function A)) : type_function_scope.
 Notation "X + Y" := (fun A : Type => sum (X%type_function A) (Y%type_function A)) : type_function_scope.
 Notation "F ∘ G" := (fun A : Type => F%type_function (G%type_function A)) : type_function_scope.
+Notation "∀ x , P" := (fun A : Type => forall x : Type, P%type_function2 A x)
+                        (at level 200, x binder, right associativity, format "∀  x ,  P") : type_function_scope.
 
 Notation "X -> Y" := (fun A B : Type => X%type_function2 A B -> Y%type_function2 A B) : type_function2_scope.
 Notation "X * Y" := (fun A B : Type => prod (X%type_function2 A B) (Y%type_function2 A B)) : type_function2_scope.
 Notation "X + Y" := (fun A B : Type => sum (X%type_function2 A B) (Y%type_function2 A B)) : type_function2_scope.
 Notation "F ∘ G" := (fun A B : Type => F%type_function2 (G%type_function2 A B)) : type_function2_scope.
+Notation "∀ x , P" := (fun A B : Type => forall x : Type, P%type_function3 A B x)
+                        (at level 200, x binder, right associativity, format "∀  x ,  P") : type_function2_scope.
+
 
 Notation "X -> Y" := (fun A B C : Type => X%type_function3 A B C -> Y%type_function3 A B C) : type_function3_scope.
 Notation "X * Y" := (fun A B C : Type => prod (X%type_function3 A B C) (Y%type_function3 A B C)) : type_function3_scope.
 Notation "X + Y" := (fun A B C : Type => sum (X%type_function3 A B C) (Y%type_function3 A B C)) : type_function3_scope.
 Notation "F ∘ G" := (fun A B C : Type => F%type_function3 (G%type_function3 A B C)) : type_function3_scope.
+Notation "∀ x , P" := (fun A B C : Type => forall x : Type, P%type_function4 A B C x)
+                        (at level 200, x binder, right associativity, format "∀  x ,  P") : type_function3_scope.
 
 Notation "X -> Y" := (fun A B C D : Type => X%type_function4 A B C D -> Y%type_function4 A B C D) : type_function4_scope.
 Notation "X * Y" := (fun A B C D : Type => prod (X%type_function4 A B C D) (Y%type_function4 A B C D)) : type_function4_scope.
